JFP-Artifact/\E/coq/Variant_Calculus.v
@@ -1,0 +1,631 @@
+(* Require Import LibTactics.
+Require Import Metalib.Metatheory.
+
+Require Import
+        syntax_ott
+        rules_inf
+        Infrastructure
+        Deterministic
+        Type_Safety
+        Typing.
+
+Require Import List. Import ListNotations.
+Require Import Arith Omega.
+Require Import Strings.String.
+
+
+Lemma fill_appl : forall e1 e2,
+  (e_app e1 e2) = (fill (appCtxL e2) e1).
+Proof.
+  intros. eauto.
+Qed.
+
+Lemma fill_appr : forall e1 e2,
+  (e_app e1 e2) = (fill (appCtxR e1) e2).
+Proof.
+  intros. eauto.
+Qed.
+
+
+Lemma fill_anno : forall e A,
+  (e_anno e A) = (fill (annoCtx A) e).
+Proof.
+  intros. eauto.
+Qed.
+
+
+Lemma eq_type: forall A,
+ (A = t_dyn) \/ ~(A = t_dyn).
+Proof.
+  introv.
+  inductions A;
+  try solve[left;
+  reflexivity];
+  try solve[right;
+  unfold not; intros H; 
+  inverts* H].
+Qed.
+
+Lemma gvalue_decidable: forall e,
+  lc_exp e -> gvalue e \/ not(gvalue e).
+Proof.
+  introv lc.
+  inductions lc; try solve[right; unfold not; intros nt; inverts* nt];
+  try solve[left*].
+  inverts IHlc.
+  - inductions H; try solve[right; unfold not; intros nt; inverts* nt];
+   try solve[left*].
+   + inductions A;try solve[right; unfold not; intros nt; inverts* nt];
+   try solve[left*].
+   right; unfold not; intros nt; inverts* nt.
+   inverts* H3.
+   + inductions A;try solve[right; unfold not; intros nt; inverts* nt];
+     try solve[left*].
+    left. eapply gvalue_fanno; eauto. reflexivity.
+   + inductions A;try solve[right; unfold not; intros nt; inverts* nt];
+    try solve[left*].
+    left. eapply gvalue_fanno; eauto. reflexivity.
+    destruct(eq_type A0);destruct(eq_type B);subst*;
+    try solve[right; unfold not; intros nt; inverts* nt; inverts* H3];
+    try solve[right; unfold not; intros nt; inverts* nt; inverts* H4];
+    try solve[left*].
+   + inductions A;try solve[right; unfold not; intros nt; inverts* nt];
+    try solve[left*].
+    right; unfold not; intros nt; inverts* nt. inverts* H5.
+    right; unfold not; intros nt; inverts* nt. inverts* H2.
+  - inductions lc; try solve[exfalso; apply H; auto];
+    try solve[right; unfold not; intros nt; inverts* nt];
+    try solve[left*].
+Qed.
+
+Theorem variant_calculus_tyred: forall v A,
+ value v -> gtyping nil (trans v) Chk A -> 
+ TypedReduce v A (Blame ) ->
+ (trans (e_anno v A) ) ->** (Blame).
+Proof.
+  introv Val Typ Red.
+  inductions Red;unfold trans in *; simpl;
+  forwards*: gtyping_regular_1 Typ; fold trans in *.
+  - inverts Typ. inverts H1. inverts H6. inverts H1.
+    inverts H4;
+    destruct B; try solve[inverts H2];
+    try solve[exfalso;apply H; auto].
+    apply gstep_b. apply gStep_annov; eauto.
+    apply gTReduce_blame.
+    unfold not; intros. inverts H1. 
+    unfold not;intros nt; inverts* nt. inverts H9. 
+  - 
+    inverts Typ. inverts H0. inverts H5. inverts H0. inverts H3; inverts H1.
+    inverts H. inverts H1. 
+    destruct(eq_type A1); destruct (eq_type A2); subst.
+    apply gstep_b. apply gStep_annov; eauto.
+    apply gvalue_dyn; eauto.
+    eapply gvalue_fanno; eauto. reflexivity.
+    apply gTReduce_blame.
+    unfold not; intros. inverts H.
+    unfold not;intros nt; inverts* nt. 
+    eapply gstep_nb. rewrite fill_anno.
+    apply gdo_step; eauto.
+    apply gStep_annov; eauto. eapply gvalue_fanno; eauto. reflexivity.
+    apply gTReduce_anyd. 
+    unfold FLike. split. unfold not; intros nt; inverts* nt.
+    split. unfold not; intros nt; inverts* nt. simpl; eauto.
+    unfold not; intros nt; inverts* nt. inverts H3. apply H1. reflexivity.
+    apply gstep_b. apply gStep_annov; eauto.
+    apply gvalue_dyn; eauto. eapply gvalue_fanno; eauto. 
+    eapply gvalue_fanno; eauto. reflexivity.
+    reflexivity.
+    apply gTReduce_blame. 
+    unfold not; intros. inverts H.
+    unfold not;intros nt; inverts* nt. 
+    eapply gstep_nb. rewrite fill_anno.
+    apply gdo_step; eauto.
+    apply gStep_annov; eauto. eapply gvalue_fanno; eauto. reflexivity.
+    apply gTReduce_anyd. 
+    unfold FLike. split. unfold not; intros nt; inverts* nt.
+    split. unfold not; intros nt; inverts* nt. simpl; eauto.
+    unfold not; intros nt; inverts* nt. inverts H3. apply H. reflexivity.
+    apply gstep_b. apply gStep_annov; eauto.
+    apply gvalue_dyn; eauto. eapply gvalue_fanno; eauto. 
+    eapply gvalue_fanno; eauto. reflexivity. reflexivity.
+    apply gTReduce_blame. 
+    unfold not; intros. inverts H1.
+    unfold not;intros nt; inverts* nt.
+    eapply gstep_nb. rewrite fill_anno.
+    apply gdo_step; eauto.
+    apply gStep_annov; eauto. 
+    eapply gvalue_fanno; eauto. reflexivity. apply gTReduce_anyd. 
+    unfold FLike. split. unfold not; intros nt; inverts* nt.
+    split. unfold not; intros nt; inverts* nt. simpl; eauto.
+    unfold not; intros nt; inverts* nt. inverts H5. apply H1. reflexivity.
+    apply gstep_b. apply gStep_annov; eauto.
+    apply gvalue_dyn; eauto. eapply gvalue_fanno; eauto. 
+    eapply gvalue_fanno; eauto. reflexivity. reflexivity.
+    apply gTReduce_blame. 
+    unfold not; intros. inverts H3.
+    unfold not;intros nt; inverts* nt.  
+Qed.
+
+
+
+Lemma lam_value_step: forall e A B C dir,
+ gtyping [] (e_anno (e_anno (e_abs (trans e)) (t_arrow A B)) t_dyn) dir C ->
+ exists v', e_anno (e_anno (e_abs (trans e)) (t_arrow A B)) t_dyn ->** (Expr v') /\ gvalue v'.
+Proof.
+  introv Typ.
+  forwards*: gtyping_regular_1 Typ. inverts H. inverts H1.
+  destruct(eq_type A);destruct(eq_type B); substs*.
+  - exists. split.
+    apply gstep_refl; eauto.
+    apply gvalue_dyn; eauto.
+    eapply gvalue_fanno; eauto. reflexivity.
+  - exists. split. 
+    eapply gstar_trans. 
+    apply gstar_one.
+    apply gStep_annov;try solve [unfold not; intros nt; inverts* nt; inverts H2; exfalso; apply 
+    H1; auto];eauto.
+    eapply gvalue_fanno; eauto. reflexivity.
+    apply gTReduce_anyd. unfold FLike.
+    split. unfold not; intros nt; inverts* nt. 
+    split. unfold not; intros nt; inverts* nt. simpl; eauto.
+    apply gstep_refl; auto. 
+    eapply gvalue_dyn; eauto.
+    eapply gvalue_fanno; eauto. 
+    eapply gvalue_fanno; eauto. reflexivity. reflexivity.
+  - exists. split. 
+    eapply gstar_trans. 
+    apply gstar_one.
+    apply gStep_annov;try solve [unfold not; intros nt; inverts* nt; inverts H2; exfalso; apply 
+    H; auto];eauto.
+    eapply gvalue_fanno; eauto. reflexivity.
+    apply gTReduce_anyd. unfold FLike.
+    split. unfold not; intros nt; inverts* nt. 
+    split. unfold not; intros nt; inverts* nt. simpl; eauto.
+    apply gstep_refl; auto. 
+    eapply gvalue_dyn; eauto.
+    eapply gvalue_fanno; eauto. 
+    eapply gvalue_fanno; eauto. reflexivity. reflexivity.
+  - exists. split. 
+    eapply gstar_trans. 
+    apply gstar_one.
+    apply gStep_annov;try solve [unfold not; intros nt; inverts* nt; inverts H3; exfalso; apply 
+    H; auto];eauto.
+    eapply gvalue_fanno; eauto. reflexivity.
+    apply gTReduce_anyd. unfold FLike.
+    split. unfold not; intros nt; inverts* nt. 
+    split. unfold not; intros nt; inverts* nt. simpl; eauto.
+    apply gstep_refl; auto. 
+    eapply gvalue_dyn; eauto.
+    eapply gvalue_fanno; eauto. 
+    eapply gvalue_fanno; eauto. reflexivity. reflexivity.
+Qed.
+
+Lemma value_gvalue:forall v dir A,
+ gtyping nil (trans v) dir A ->
+ value v ->
+ exists v', (trans v) ->** (Expr v') /\ gvalue v'.
+Proof.
+  introv typ val. gen A.
+  inductions val; intros;simpl.
+  - destruct A.
+    + exists. split. apply gstar_one; eauto.
+      apply gStep_annov;try solve [unfold not; intros nt; inverts* nt];eauto. eauto.
+    + inverts* typ. inverts* H4; inverts H; inverts H0. inverts H. inverts H4. inverts H; inverts H2.
+    + exists. split*.
+  - destruct C.
+    + inverts typ. inverts H5. inverts H0; inverts H1.
+      inverts H0. inverts H5. inverts H0; inverts H3.
+    + forwards*: gtyping_regular_1 typ. inverts H0. inverts H2.
+      exists. split*. eapply gvalue_fanno; eauto. 
+      eapply gvalue_fanno; eauto. reflexivity. reflexivity.
+    + simpl in *. 
+       forwards*: lam_value_step typ.
+Qed.
+
+
+
+Lemma Tred_value: forall v v' A,
+  gvalue v->
+  gTypedReduce v A (Expr v') ->
+  gvalue v'.
+Proof.
+  introv Val Red.
+  inductions Red; eauto.
+  - apply gvalue_dyn; eauto.
+    inverts H.
+    inverts H1.
+    inverts Val; inverts* H2.
+    eapply gvalue_fanno; eauto.
+    reflexivity.
+  - inverts* Val.
+    inverts H.
+    inverts H4.
+    inverts* H5.
+    inverts* H0.
+    rewrite <- H5 in H2.
+    inverts H2.
+  - inverts* Val.
+Qed.
+
+
+
+Lemma typlist3_typlist4: forall v A3 A1, 
+ value v ->
+ TypeLists v [A3; t_dyn; A1] Blame ->
+ TypeLists v [A3; A1] Blame.
+Proof.
+  introv val tl.
+  inverts tl;try solve[inverts val]; try solve[inverts H10]. inverts H5.  inverts H8; try solve[inverts H10].
+  forwards*: TypedReduce_prv_value H3. forwards*: value_lc H.
+  forwards*: TypedReduce_prv_value H6. forwards*: value_lc H7.
+  forwards*: TypedReduce_transr H6 H5.
+  forwards*: TypedReduce_prv_value H3. 
+  forwards*: TypedReduce_transr H6 H7.
+  inverts H6. exfalso; apply H; eauto.
+  apply TLists_consb; eauto.
+Qed.
+
+
+Lemma gvalue_lc : forall v,
+    gvalue v -> lc_exp v.
+Proof.
+  intros v H.
+  induction* H. 
+Qed.
+
+Lemma lam_value_red: forall v A B ,
+ gvalue v ->
+ principal_type v = t_arrow A B ->
+ e_anno v t_dyn ->** (Expr (e_anno v  t_dyn)) /\ gvalue (e_anno v t_dyn) /\ (t_arrow A B = t_arrow t_dyn t_dyn) \/
+ e_anno v t_dyn ->** (Expr (e_anno (e_anno v (t_arrow t_dyn t_dyn)) t_dyn)) /\ gvalue (e_anno (e_anno v (t_arrow t_dyn t_dyn)) t_dyn).
+Proof.
+  introv val typ.
+  forwards*: gvalue_lc val. inverts val; try solve[inverts* typ]. inverts typ.
+  + destruct(eq_type A);destruct(eq_type B); substs*.
+  - right. split. 
+    eapply gstar_trans. 
+    apply gstar_one.
+    apply gStep_annov;try solve [unfold not; intros nt; inverts* nt; inverts H3; exfalso; apply 
+    H1; auto];eauto.
+    apply gTReduce_anyd. unfold FLike.
+    split. unfold not; intros nt; inverts* nt. 
+    split. unfold not; intros nt; inverts* nt. simpl; eauto.
+    unfold not; intros nt; inverts* nt. inverts* H4.
+    apply gstep_refl; auto. 
+    eapply gvalue_dyn; eauto.
+    eapply gvalue_fanno; eauto.  reflexivity.
+  - right. split. 
+  eapply gstar_trans. 
+  apply gstar_one.
+  apply gStep_annov;try solve [unfold not; intros nt; inverts* nt; inverts H2; exfalso; apply 
+  H1; auto];eauto.
+  apply gTReduce_anyd. unfold FLike.
+  split. unfold not; intros nt; inverts* nt. 
+  split. unfold not; intros nt; inverts* nt. simpl; eauto.
+  unfold not; intros nt; inverts* nt. inverts* H4.
+  apply gstep_refl; auto. 
+  eapply gvalue_dyn; eauto.
+  eapply gvalue_fanno; eauto.  reflexivity.
+  - right. split. 
+  eapply gstar_trans. 
+  apply gstar_one.
+  apply gStep_annov;try solve [unfold not; intros nt; inverts* nt; inverts H2; exfalso; apply 
+  H1; auto];eauto.
+  apply gTReduce_anyd. unfold FLike.
+  split. unfold not; intros nt; inverts* nt. 
+  split. unfold not; intros nt; inverts* nt. simpl; eauto.
+  unfold not; intros nt; inverts* nt. inverts* H5.
+  apply gstep_refl; auto. 
+  eapply gvalue_dyn; eauto.
+  eapply gvalue_fanno; eauto.  reflexivity.
+Qed.
+
+
+Lemma lam_value_tred: forall v A B ,
+ gvalue v ->
+ principal_type v = t_arrow A B ->
+ gTypedReduce v t_dyn (Expr (e_anno v t_dyn)) /\ gvalue (e_anno v t_dyn) \/
+ gTypedReduce v t_dyn (Expr (e_anno (e_anno v (t_arrow t_dyn t_dyn)) t_dyn)) /\ gvalue (e_anno (e_anno v (t_arrow t_dyn t_dyn)) t_dyn).
+Proof.
+  introv val typ.
+  forwards*: gvalue_lc val. inverts val;inverts* typ. 
+  + destruct(eq_type A);destruct(eq_type B); substs*.
+  - right. split. 
+    apply gTReduce_anyd. unfold FLike.
+    split. unfold not; intros nt; inverts* nt. 
+    split. unfold not; intros nt; inverts* nt. simpl; eauto.
+    eapply gvalue_dyn; eauto.
+    eapply gvalue_fanno; eauto.  reflexivity.
+  - right. split. 
+    apply gTReduce_anyd. unfold FLike.
+    split. unfold not; intros nt; inverts* nt. 
+    split. unfold not; intros nt; inverts* nt. simpl; eauto.
+    eapply gvalue_dyn; eauto.
+    eapply gvalue_fanno; eauto.  reflexivity.
+  - right. split. 
+    apply gTReduce_anyd. unfold FLike.
+    split. unfold not; intros nt; inverts* nt. 
+    split. unfold not; intros nt; inverts* nt. simpl; eauto.
+    eapply gvalue_dyn; eauto.
+    eapply gvalue_fanno; eauto.  reflexivity.
+Qed.
+
+
+
+Lemma typlist_gtyplist: forall v A0 A1,
+  value v ->
+  lc_exp (trans v) ->
+  gtyping [] (trans v) Chk A0 ->
+  TypeLists v [ A0; A1] (Blame) ->
+  sim A0 A1 ->
+  exists v', (trans v) ->** (Expr v') /\ gvalue v' /\ gTypeLists v' [ A0; A1] Blame.
+Proof.
+  introv val lc typ typlist sim.
+  inverts typlist.
+  - inverts H5; try solve[inverts H8].
+    + (* a1 blame *)
+      inverts val;inverts H3; inverts* H4;try solve[inverts H6]; try solve[inverts sim]; simpl in *.
+      * (* i:a0 *)
+        inverts typ. inverts H. inverts H10. inverts H.
+        inverts H4. inverts H2; try solve[exfalso; apply H5; auto]. 
+        (* i:int-> a0 a1 *)
+        exists. split. apply gstar_one; eauto.
+        apply gStep_annov;try solve [unfold not; intros nt; inverts* nt];eauto. split*. 
+        eapply gTLists_cons; auto.
+        assert(not(syntax_ott.sim A1 t_int)). unfold not; intros nt. apply H5. apply BA_AB; auto.
+        eapply gTLists_consb; auto.
+        (* i:dyn-> a0 a1 *)
+        inverts* H9.
+        exists. split. apply gstep_refl; eauto.
+        split*. 
+        eapply gTLists_cons; auto.
+        assert(not(syntax_ott.sim A1 t_int)). unfold not; intros nt. apply H5. apply BA_AB; auto.
+        eapply gTLists_consb; auto.
+      *
+        inverts lc. inverts H3.
+        inverts typ. inverts H2. inverts H11. inverts H2.
+        inverts sim; inverts H10.
+        inverts H6.
+        assert(gvalue((e_anno (e_anno (e_abs (trans e)) (t_arrow A B)) (t_arrow C D)))).
+        eapply gvalue_fanno; eauto. eapply gvalue_fanno;eauto. reflexivity. reflexivity.
+        forwards*: lam_value_tred H2. inverts H6. inverts H10.
+        exists. split. apply gstep_refl; eauto.
+        split*.
+        eapply gTLists_cons; auto.
+        apply H6.
+        eapply gTLists_baseb; eauto.
+        apply gTReduce_blame;try solve [unfold not; intros nt; inverts* nt];eauto.
+        inverts H10.
+        exists. split. apply gstep_refl; eauto.
+        split*.
+        eapply gTLists_cons; auto.
+        apply H6.
+        eapply gTLists_baseb; eauto.
+        apply gTReduce_blame;try solve [unfold not; intros nt; inverts* nt];eauto.
+        
+        assert(gvalue(e_anno (e_abs (trans e)) (t_arrow A B))).
+        eapply gvalue_fanno; eauto. reflexivity.
+        forwards*: lam_value_red H2. inverts H6. inverts H10. inverts H11. inverts H12.
+        exists. split. apply H6.
+        split*.
+        eapply gTLists_cons; auto.
+        eapply gTLists_baseb; eauto.
+        apply gTReduce_blame;try solve [unfold not; intros nt; inverts* nt];eauto.
+        inverts H10.
+        exists. split. apply H6.
+        split*.
+        eapply gTLists_cons; auto.
+        eapply gTLists_baseb; eauto.
+        apply gTReduce_blame;try solve [unfold not; intros nt; inverts* nt];eauto.
+    + inverts val; inverts H3; inverts* H6;try solve[inverts* H5];try solve[inverts sim]; simpl in *.
+      * (* i:a0 *)
+        inverts typ. inverts H. inverts H10. inverts H.
+        inverts H6. inverts H0; try solve[exfalso; apply H3; auto]. 
+        (* i:int-> a0 a1 *)
+        exists. split. apply gstar_one; eauto.
+        apply gStep_annov;try solve [unfold not; intros nt; inverts* nt];eauto. split*. 
+        eapply gTLists_cons; auto.
+        assert(not(syntax_ott.sim A1 t_int)). unfold not; intros nt. apply H3. apply BA_AB; auto.
+        eapply gTLists_consb; auto.
+        (* i:dyn-> a0 a1 *)
+        inverts* H9.
+        exists. split. apply gstep_refl; eauto.
+        split*. 
+        eapply gTLists_cons; auto.
+        assert(not(syntax_ott.sim A1 t_int)). unfold not; intros nt. apply H3. apply BA_AB; auto.
+        eapply gTLists_consb; auto.
+      *
+        inverts lc. inverts H2.
+        inverts typ. inverts H0. inverts H11. inverts H0.
+        inverts sim; inverts H10.
+        inverts H6. 
+        assert(gvalue((e_anno (e_anno (e_abs (trans e)) (t_arrow A B)) (t_arrow C D)))).
+        eapply gvalue_fanno; eauto. eapply gvalue_fanno;eauto. reflexivity. reflexivity.
+        forwards*: lam_value_tred H0. inverts H6. inverts H10.
+        exists. split. apply gstep_refl; eauto.
+        split*.
+        eapply gTLists_cons; auto.
+        apply H6.
+        eapply gTLists_baseb; eauto.
+        apply gTReduce_blame;try solve [unfold not; intros nt; inverts* nt];eauto.
+        inverts H10.
+        exists. split. apply gstep_refl; eauto.
+        split*.
+        eapply gTLists_cons; auto.
+        apply H6.
+        eapply gTLists_baseb; eauto.
+        apply gTReduce_blame;try solve [unfold not; intros nt; inverts* nt];eauto.
+        
+        assert(gvalue(e_anno (e_abs (trans e)) (t_arrow A B))).
+        eapply gvalue_fanno; eauto. reflexivity.
+        forwards*: lam_value_red H0. inverts H6. inverts H10. inverts H11. inverts H12.
+        exists. split. apply H6.
+        split*.
+        eapply gTLists_cons; auto.
+        eapply gTLists_baseb; eauto.
+        apply gTReduce_blame;try solve [unfold not; intros nt; inverts* nt];eauto.
+        inverts H10.
+        exists. split. apply H6.
+        split*.
+        eapply gTLists_cons; auto.
+        eapply gTLists_baseb; eauto.
+        apply gTReduce_blame;try solve [unfold not; intros nt; inverts* nt];eauto.
+  - 
+    inverts val; inverts typ; simpl in *.
+    +
+    inverts H3.
+    inverts* H. inverts H5. inverts H. inverts H3; try solve[exfalso; apply H7; auto].
+    exists. split. 
+    apply gstep_refl; eauto.
+    split*.
+    eapply gTLists_consb; auto.
+    apply gTReduce_blame;try solve [unfold not; intros nt; inverts* nt];eauto.
+    +
+    inverts H0. inverts H7. inverts H0. inverts H3. inverts H1; inverts H5.
+    forwards*: gtyping_regular_1 H9.
+    assert(gvalue((e_anno (e_abs (trans e)) (t_arrow A B)))).
+    eapply gvalue_fanno; eauto.  reflexivity.
+    forwards*: lam_value_red H1. inverts H3. inverts H5. inverts H7. inverts H8.
+    exists. split. apply gstep_refl; eauto.
+    split*.
+    eapply gTLists_consb; eauto.
+    apply gTReduce_blame;try solve [unfold not; intros nt; inverts* nt];eauto.
+    inverts H5.
+    exists. split. apply H3.
+    split*.
+    eapply gTLists_consb; eauto.
+    apply gTReduce_blame;try solve [unfold not; intros nt; inverts* nt];eauto.
+Qed.
+
+
+
+Lemma glist_blame: forall e x A0 A1 A B1,
+ gvalue x ->
+ lc_exp (e_abs e) ->
+ gTypeLists x [A0; A1] Blame ->
+ e_app (e_anno (e_anno (e_abs e) (t_arrow A1 B1)) (t_arrow A0 A)) x ->** Blame.
+Proof.
+  introv val lc ls.
+  inverts ls. inverts H5.
+  -
+    eapply gstar_transb.
+    apply gstar_one.
+    apply gStep_abeta; eauto.
+    eapply gvalue_fanno;eauto. reflexivity.
+    rewrite fill_anno.
+    apply gstep_b.
+    apply gblame_step;eauto.
+    apply gStep_betap; eauto.
+    eapply gvalue_fanno;eauto. reflexivity.
+    forwards*: Tred_value H3.
+  -
+    inverts H8.
+  -
+    eapply gstar_transb.
+    apply gstar_one.
+    apply gStep_abeta; eauto.
+    eapply gvalue_fanno;eauto. reflexivity.
+    rewrite fill_anno.
+    apply gstep_b.
+    apply gblame_step;eauto.
+    apply gStep_betap; eauto.
+    eapply gvalue_fanno;eauto. reflexivity.
+    forwards*: Tred_value H3.
+  -
+    apply gstep_b.
+    apply gStep_betap; eauto.
+    eapply gvalue_fanno;eauto. eapply gvalue_fanno;eauto. reflexivity. reflexivity.
+Qed.
+
+
+
+
+Theorem variant_calculus: forall e dir A,
+ gtyping nil (trans e) dir A -> step e Blame 
+ -> (trans e) ->** Blame.
+Proof with eauto.
+  introv Typ Red. gen dir A.
+    inductions Red; intros; eauto; unfold trans; simpl;
+    forwards*: gtyping_regular_1 Typ; fold trans.
+  - destruct E; unfold simpl_fill in *; inverts* Typ.
+    + forwards*: IHRed H4. inverts H0.
+      apply multi_blame_app2...
+    + inverts* H0. inverts H1. forwards*: IHRed H8. inverts H. 
+      apply multi_blame_app2 ...
+    + forwards*: IHRed H7. inverts H;simpl.
+      inverts H3.
+      forwards*: value_gvalue H. inverts H2. inverts H3.
+      eapply gstar_transb.
+      apply gmulti_red_app2... inverts* H0.
+       apply multi_blame_app; eauto.
+       eapply gstar_transb.
+       apply gmulti_red_app2... inverts* H0.
+        apply multi_blame_app; eauto.
+      forwards*: gtyping_regular_1 H4.
+        simpl; auto.
+    + inverts* H0. inverts H1. forwards*: IHRed H9. inverts H; simpl.
+      inverts H4.
+       forwards*: value_gvalue H. inverts H1. inverts H4.
+      eapply gstar_transb.
+      apply gmulti_red_app2... 
+       apply multi_blame_app; eauto.
+       eapply gstar_transb.
+       apply gmulti_red_app2... 
+        apply multi_blame_app; eauto.
+       forwards*: gtyping_regular_1 H8.
+       simpl; auto.
+    + inverts* H1.
+    + inverts* H1.
+  - inverts* Typ. forwards*: IHRed H6. 
+    + apply multi_blame_anno; eauto.
+    + inverts H1. forwards*: IHRed H6. 
+      apply multi_blame_anno; eauto.
+  -
+     inverts Typ.
+     *
+     inverts H6.
+     forwards*: gtyping_regular_1 H9. inverts H8. 
+     inverts H4; inverts H5.
+     forwards*: gtyping_regular_1 H10.
+     apply BA_AB in H11. 
+     forwards*: typlist_gtyplist H1.
+     inverts H5. inverts H7. inverts H8.
+     eapply gstar_transb.
+     eapply gmulti_red_app.
+     eapply gvalue_fanno;eauto. eapply gvalue_fanno; eauto. reflexivity. reflexivity.
+     apply H5.
+     forwards*: glist_blame H7 H12.
+     *
+     inverts H3. inverts H9.
+     forwards*: gtyping_regular_1 H10. inverts H11. inverts H6; inverts H7.
+     apply BA_AB in H13.
+     forwards*: gtyping_regular_1 H12.
+     forwards*: typlist_gtyplist H1.
+     inverts H7. inverts H9. inverts H11. 
+     eapply gstar_transb.
+     eapply gmulti_red_app.
+     eapply gvalue_fanno;eauto. eapply gvalue_fanno; eauto. reflexivity. reflexivity.
+     apply H7.
+     forwards*: glist_blame H9 H14.
+  - 
+   inverts H1.
+   inverts Typ. 
+   + 
+      forwards*: variant_calculus_tyred H0.
+   + inverts H1.
+      forwards*: variant_calculus_tyred H0.
+  - inverts* Typ. inverts* H3. 
+  - inverts* Typ. inverts* H2.
+Qed.
+
+
+
+(* 
+Theorem variant_calculus_final: forall e dir A,
+ gtyping nil (trans e) dir A -> e ->* Blame 
+ -> (trans e) ->** Blame.
+Proof with eauto.
+ introv typ red1. gen dir A.
+ inductions red1; intros.
+ - forwards*: variant_calculus H.
+Qed. *) *)
